theories/LambdaSep.v
@@ -412,46 +412,6 @@ Proof using.
   exists h' v. splits~. { hhsimpl. auto. }
 Qed.
 
-Lemma hoare_hexists : forall t (A:Type) (J:A->hprop) Q,
-  (forall x, hoare t (J x) Q) ->
-  hoare t (hexists J) Q.
-Proof using. introv M (x&Hh). applys* M. Qed.
-
-Lemma hoare_hforall : forall t (A:Type) (J:A->hprop) Q,
-  (exists x, hoare t (J x) Q) ->
-  hoare t (hforall J) Q.
-Proof using. introv (x&M) Hh. applys* M. Qed.
-
-Lemma hoare_hprop : forall t (P:Prop) H Q,
-  (P -> hoare t H Q) ->
-  hoare t (\[P] \* H) Q.
-Proof using.
-  introv M. applys~ triple_hprop_from_hexists.
-  { applys* hoare_hexists. }
-Qed.
-(* Details:
-  introv M (h1&h2&N1&N2&N3&N4).
-  destruct (hpure_inv' N1). subst.
-  rewrite heap_union_empty_l.
-  applys* M.
-*)
-
-Lemma hoare_hwand_hpure_l : forall t (P:Prop) H Q,
-  P ->
-  hoare t H Q ->
-  hoare t (\[P] \-* H) Q.
-Proof using.
-  introv HP M. applys~ triple_hwand_hpure_l_from_hexists_and_consequence.
-  { applys* hoare_hexists. }
-  { introv N W. applys* hoare_conseq. }
-Qed.
-(* Details:
-  introv HP M. intros h (H1&(h1&h2&N1&N2&N3&N4)).
-  lets (N2'&E): (hpure_inv' (rm N2)). subst.
-  rewrite heap_union_empty_r.
-  applys* M. applys N2'. hhsimpl~.
-*)
-
 Lemma hoare_named_heap : forall t H Q,
   (forall h, H h -> hoare t (= h) Q) ->
   hoare t H Q.
@@ -699,28 +659,22 @@ End HoarePrimitives.
 Definition triple (t:trm) (H:hprop) (Q:val->hprop) :=
   forall H', hoare t (H \* H') (Q \*+ H' \*+ \Top).
 
-(** SL triples are "local", in the sense of SepFunctor *)
+(** SL triples satisfy [is_local], in the sense of SepFunctor *)
 
 Lemma is_local_triple : forall t,
   is_local (triple t).
 Proof using.
-  intros. applys pred_ext_2. intros H Q. iff M.
-  { intros h Hh. hhsimpl. split*. hsimpl. }
-  { intros H'. applys hoare_named_heap.
-    intros h (h1&h2&N1&N2&N3&N4).
-    lets (H1&H2&Q1&M0): (rm M) (rm N1).
-    rewrite <-hstar_assoc, hstar_comm, hstar_pure in M0.
-    destruct M0 as ((M1&M2)&M3).
-    applys hoare_conseq (M1 (H2 \* H')).
-    { subst. rewrite <- hstar_assoc. intros h ->. apply~ hstar_intro. }
-    { intros x. hchanges (M2 x). } }
+  intros. applys is_local_intro. intros H Q M H'. 
+  applys hoare_named_heap. intros h (h1&h2&N1&N2&N3&N4).
+  lets (H1&H2&Q1&M0): (rm M) (rm N1).
+  rewrite <- hstar_assoc, hstar_comm, hstar_pure in M0.
+  destruct M0 as ((M1&M2)&M3).
+  applys hoare_conseq (M1 (H2 \* H')).
+  { subst. rewrite <- hstar_assoc. intros h ->. apply~ hstar_intro. }
+  { intros x. hchanges (M2 x). }
 Qed.
 
-(** Make tactic [xlocal] aware that triples are local *)
-
-Ltac xlocal_base tt ::=
-  try first [ applys is_local_local
-            | applys is_local_triple ].
+Hint Resolve is_local_triple.
 
 (** Lemma to introduce hoare instances for establishing triples,
     integrating the consequence rule. *)
@@ -750,107 +704,71 @@ Lemma triple_conseq : forall t H' Q' H Q,
   H ==> H' ->
   Q' ===> Q ->
   triple t H Q.
-Proof using.
-  introv M MH MQ. intros HF. applys hoare_conseq M.
-  { hchanges MH. }
-  { intros x. hchanges (MQ x). }
-Qed.
+Proof using. intros. applys* is_local_conseq. Qed.
+
+Lemma triple_frame : forall t H Q H',
+  triple t H Q ->
+  triple t (H \* H') (Q \*+ H').
+Proof using. intros. applys* is_local_frame. Qed.
+
+Lemma triple_htop_pre : forall t H Q,
+  triple t H Q ->
+  triple t (H \* \Top) Q.
+Proof using. intros. applys* is_local_htop_pre. Qed.
+
+Lemma triple_htop_post : forall t H Q,
+  triple t H (Q \*+ \Top) ->
+  triple t H Q.
+Proof using. intros. applys* is_local_htop_post. Qed.
 
 Lemma triple_hexists : forall t (A:Type) (J:A->hprop) Q,
   (forall x, triple t (J x) Q) ->
   triple t (hexists J) Q.
-Proof using.
-  introv M. intros HF. rewrite hstar_hexists.
-  applys hoare_hexists. intros. applys* M.
-Qed.
+Proof using. intros. applys* is_local_hexists. Qed.
 
-Lemma triple_hforall : forall t A (J:A->hprop) Q,
-  (exists x, triple t (J x) Q) ->
-  triple t (hforall J) Q.
-Proof using.
-  introv (x&M). intros HF.
-  forwards* N: hoare_hforall (fun x => J x \* HF).
-  applys* hoare_conseq. applys hstar_hforall.
-Qed.
-
-Lemma triple_hforall_for : forall A (x:A) t (J:A->hprop) Q,
+Lemma triple_hforall : forall A (x:A) t (J:A->hprop) Q,
   triple t (J x) Q ->
   triple t (hforall J) Q.
-Proof using. intros. applys* triple_hforall. Qed.
+Proof using. intros. applys* is_local_hforall. Qed.
+
+Lemma triple_hforall_exists : forall t A (J:A->hprop) Q, (* TODO: needed?*)
+  (exists x, triple t (J x) Q) ->
+  triple t (hforall J) Q.
+Proof using. intros. applys* is_local_hforall_exists. Qed.
 
 Lemma triple_hprop : forall t (P:Prop) H Q,
   (P -> triple t H Q) ->
   triple t (\[P] \* H) Q.
-Proof using.
-  introv M. intros HF. rewrite hstar_assoc.
-  applys hoare_hprop. intros. applys* M.
-Qed.
+Proof using. intros. applys* is_local_hprop. Qed.
 
 Lemma triple_hwand_hpure_l : forall t (P:Prop) H Q,
   P ->
   triple t H Q ->
   triple t (\[P] \-* H) Q.
-Proof using.
-  introv HP M. intros HF.
-  forwards* N: hoare_hwand_hpure_l P.
-  applys* hoare_conseq. applys hstar_hwand.
-Qed.
+Proof using. intros. applys* is_local_hwand_hpure_l. Qed.
 
 Lemma triple_hor : forall t H1 H2 Q,
   triple t H1 Q ->
   triple t H2 Q ->
   triple t (hor H1 H2) Q.
-Proof using.
-  introv M1 M2. unfold hor. applys triple_hexists.
-  intros b. destruct* b.
-Qed.
+Proof using. intros. applys* is_local_hor. Qed.
 
 Lemma triple_hand_l : forall t H1 H2 Q,
   triple t H1 Q ->
   triple t (hand H1 H2) Q.
-Proof using.
-  introv M1. unfold hand. applys triple_hforall. exists* true.
-Qed.
+Proof using. intros. applys* is_local_hand_l. Qed.
 
 Lemma triple_hand_r : forall t H1 H2 Q,
   triple t H2 Q ->
   triple t (hand H1 H2) Q.
-Proof using.
-  introv M1. unfold hand. applys triple_hforall. exists* false.
-Qed.
+Proof using. intros. applys* is_local_hand_r. Qed.
 
-Lemma triple_frame : forall t H Q H',
-  triple t H Q ->
-  triple t (H \* H') (Q \*+ H').
-Proof using.
-  introv M. intros HF.
-  applys hoare_conseq (M (HF \* H')); hsimpl.
-Qed.
-
-Lemma triple_htop_post : forall t H Q,
-  triple t H (Q \*+ \Top) ->
-  triple t H Q.
-Proof using.
-  introv M. intros HF.
-  applys hoare_conseq (M HF); hsimpl.
-Qed.
-
-Lemma triple_htop_pre : forall t H Q,
-  triple t H Q ->
-  triple t (H \* \Top) Q.
-Proof using.
-  introv M. applys triple_htop_post. applys~ triple_frame.
-Qed.
-
-Lemma triple_combined : forall H2 H1 Q1 t H Q,
+Lemma triple_conseq_frame_htop : forall H2 H1 Q1 t H Q,
   triple t H1 Q1 ->
   H ==> H1 \* H2 ->
   Q1 \*+ H2 ===> Q \*+ \Top ->
   triple t H Q.
-Proof using.
-  introv M WH WQ. applys triple_htop_post. applys triple_conseq.
-  { applys* triple_frame. } { eauto. } { eauto. }
-Qed.
+Proof using. intros. applys* is_local_conseq_frame_htop. Qed.
 
 
 (* ---------------------------------------------------------------------- *)
@@ -1034,8 +952,9 @@ Lemma triple_while_inv : forall (A:Type) (I:bool->A->hprop) (R:A->A->Prop) H' t1
   Q' \*+ H' ===> Q \*+ \Top ->
   triple (trm_while t1 t2) H Q.
 Proof using.
-  introv WR WH HX WQ. applys triple_combined WH WQ. xpull ;=> b0 X0.
-  gen b0. induction_wf IH: WR X0. intros. applys triple_while_raw.
+  introv WR WH HX WQ. applys triple_conseq_frame_htop WH WQ.
+  xpull ;=> b0 X0. gen b0. induction_wf IH: WR X0.
+  intros. applys triple_while_raw.
   applys HX. intros b' X' HR'. applys~ IH.
 Qed.
 
