theories/LambdaSepAltProofs.v
@@ -1,0 +1,314 @@
+
+Set Implicit Arguments.
+From Sep Require LambdaSep LambdaSepLifted.
+
+
+(* ********************************************************************** *)
+(* * Additional lemmas *)
+
+(* ---------------------------------------------------------------------- *)
+(* ** Auxiliary lemma showing that reasoning rule for extracting
+   pure propositions from preconditions is just a special case
+   of the reasoning rule for extracting existentials from preconditions. *)
+
+Lemma triple_hprop_from_hexists :
+  forall (T:Type) (F:hprop->(T->hprop)->Prop),
+  (forall (A:Type) (J:A->hprop) (Q:T->hprop),
+    (forall x, F (J x) Q) ->
+    F (hexists J) Q) ->
+  (forall P H Q,
+    (P -> F H Q) ->
+    F (\[P] \* H) Q).
+Proof using.
+  introv M. introv N. rewrite hpure_eq_hexists_empty.
+  rewrite hstar_hexists.
+  applys M. rewrite~ hstar_hempty_l.
+Qed.
+
+Arguments triple_hprop_from_hexists [T].
+
+Lemma triple_hwand_hpure_l_from_hexists_and_consequence :
+  forall (T:Type) (F:hprop->(T->hprop)->Prop),
+  (forall (A:Type) (J:A->hprop) (Q:T->hprop),
+    (forall x, F (J x) Q) ->
+    F (hexists J) Q) ->
+  (forall H1 H2 (Q:T->hprop),
+    F H1 Q ->
+    H2 ==> H1 ->
+    F H2 Q) ->
+  (forall P H Q,
+    P ->
+    F H Q ->
+    F (\[P] \-* H) Q).
+Proof using.
+  introv M W HP. introv N. rewrite hwand_eq_hexists_hstar_hpure.
+  applys M. intros. applys* W. hpull. introv R. hchanges~ R.
+Qed.
+
+
+
+(* ********************************************************************** *)
+(* * Additional proofs for structural rules of LambdaSep's [hoare] triples *)
+
+Module LambdaSepAlt.
+Import LambdaSep.
+
+Lemma hoare_hexists : forall t (A:Type) (J:A->hprop) Q,
+  (forall x, hoare t (J x) Q) ->
+  hoare t (hexists J) Q.
+Proof using. introv M (x&Hh). applys* M. Qed.
+
+Lemma hoare_hforall : forall t (A:Type) (J:A->hprop) Q,
+  (exists x, hoare t (J x) Q) ->
+  hoare t (hforall J) Q.
+Proof using. introv (x&M) Hh. applys* M. Qed.
+
+Lemma hoare_hprop : forall t (P:Prop) H Q,
+  (P -> hoare t H Q) ->
+  hoare t (\[P] \* H) Q.
+Proof using.
+  introv M. applys~ triple_hprop_from_hexists.
+  { applys* hoare_hexists. }
+Qed.
+(* Details:
+  introv M (h1&h2&N1&N2&N3&N4).
+  destruct (hpure_inv' N1). subst.
+  rewrite heap_union_empty_l.
+  applys* M.
+*)
+
+Lemma hoare_hwand_hpure_l : forall t (P:Prop) H Q,
+  P ->
+  hoare t H Q ->
+  hoare t (\[P] \-* H) Q.
+Proof using.
+  introv HP M. applys~ triple_hwand_hpure_l_from_hexists_and_consequence.
+  { applys* hoare_hexists. }
+  { introv N W. applys* hoare_conseq. }
+Qed.
+(* Details:
+  introv HP M. intros h (H1&(h1&h2&N1&N2&N3&N4)).
+  lets (N2'&E): (hpure_inv' (rm N2)). subst.
+  rewrite heap_union_empty_r.
+  applys* M. applys N2'. hhsimpl~.
+*)
+
+
+
+(* ********************************************************************** *)
+(* * Alternative proofs for structural rules of LambdaSep's SL [triple] *)
+
+Implicit Types H : hprop.
+Implicit Types Q : val -> hprop.
+
+Lemma triple_conseq : forall t H' Q' H Q,
+  triple t H' Q' ->
+  H ==> H' ->
+  Q' ===> Q ->
+  triple t H Q.
+Proof using.
+  introv M MH MQ. intros HF. applys hoare_conseq M.
+  { hchanges MH. }
+  { intros x. hchanges (MQ x). }
+Qed.
+
+Lemma triple_hexists : forall t (A:Type) (J:A->hprop) Q,
+  (forall x, triple t (J x) Q) ->
+  triple t (hexists J) Q.
+Proof using.
+  introv M. intros HF. rewrite hstar_hexists.
+  applys hoare_hexists. intros. applys* M.
+Qed.
+
+Lemma triple_hforall : forall t A (J:A->hprop) Q,
+  (exists x, triple t (J x) Q) ->
+  triple t (hforall J) Q.
+Proof using.
+  introv (x&M). intros HF.
+  forwards* N: hoare_hforall (fun x => J x \* HF).
+  applys* hoare_conseq. applys hstar_hforall.
+Qed.
+
+(** corrolary *)
+Lemma triple_hforall_for : forall A (x:A) t (J:A->hprop) Q,
+  triple t (J x) Q ->
+  triple t (hforall J) Q.
+Proof using. intros. applys* triple_hforall. Qed.
+
+Lemma triple_hprop : forall t (P:Prop) H Q,
+  (P -> triple t H Q) ->
+  triple t (\[P] \* H) Q.
+Proof using.
+  introv M. intros HF. rewrite hstar_assoc.
+  applys hoare_hprop. intros. applys* M.
+Qed.
+
+Lemma triple_hwand_hpure_l : forall t (P:Prop) H Q,
+  P ->
+  triple t H Q ->
+  triple t (\[P] \-* H) Q.
+Proof using.
+  introv HP M. intros HF.
+  forwards* N: hoare_hwand_hpure_l P.
+  applys* hoare_conseq. applys hstar_hwand.
+Qed.
+
+Lemma triple_hor : forall t H1 H2 Q,
+  triple t H1 Q ->
+  triple t H2 Q ->
+  triple t (hor H1 H2) Q.
+Proof using.
+  introv M1 M2. unfold hor. applys triple_hexists.
+  intros b. destruct* b.
+Qed.
+
+Lemma triple_hand_l : forall t H1 H2 Q,
+  triple t H1 Q ->
+  triple t (hand H1 H2) Q.
+Proof using.
+  introv M1. unfold hand. applys triple_hforall. exists* true.
+Qed.
+
+Lemma triple_hand_r : forall t H1 H2 Q,
+  triple t H2 Q ->
+  triple t (hand H1 H2) Q.
+Proof using.
+  introv M1. unfold hand. applys triple_hforall. exists* false.
+Qed.
+
+Lemma triple_frame : forall t H Q H',
+  triple t H Q ->
+  triple t (H \* H') (Q \*+ H').
+Proof using.
+  introv M. intros HF.
+  applys hoare_conseq (M (HF \* H')); hsimpl.
+Qed.
+
+Lemma triple_htop_post : forall t H Q,
+  triple t H (Q \*+ \Top) ->
+  triple t H Q.
+Proof using.
+  introv M. intros HF.
+  applys hoare_conseq (M HF); hsimpl.
+Qed.
+
+Lemma triple_htop_pre : forall t H Q,
+  triple t H Q ->
+  triple t (H \* \Top) Q.
+Proof using.
+  introv M. applys triple_htop_post. applys~ triple_frame.
+Qed.
+
+Lemma triple_combined : forall H2 H1 Q1 t H Q,
+  triple t H1 Q1 ->
+  H ==> H1 \* H2 ->
+  Q1 \*+ H2 ===> Q \*+ \Top ->
+  triple t H Q.
+Proof using.
+  introv M WH WQ. applys triple_htop_post. applys triple_conseq.
+  { applys* triple_frame. } { eauto. } { eauto. }
+Qed.
+
+End LambdaSepAlt.
+
+
+(* ********************************************************************** *)
+(* * Alternative proofs for structural rules of LambdaSep's SL [triple] *)
+
+Module LambdaSepLiftedAlt.
+Implicit Types H : hprop.
+
+Lemma Triple_conseq : forall t H' `{Enc A} (Q':A->hprop) H (Q:A->hprop),
+  H ==> H' ->
+  Triple t H' Q' ->
+  Q' ===> Q ->
+  Triple t H Q.
+Proof using. introv MH M MQ. applys* triple_conseq MH. Qed.
+
+Lemma Triple_hexists : forall t `{Enc A} B (J:B->hprop) (Q:A->hprop),
+  (forall x, Triple t (J x) Q) ->
+  Triple t (hexists J) Q.
+Proof using. intros. applys~ triple_hexists. Qed.
+
+Lemma Triple_hforall : forall t B (J:B->hprop) `{EA:Enc A} (Q:A->hprop),
+  (exists x, Triple t (J x) Q) ->
+  Triple t (hforall J) Q.
+Proof using. unfold Triple. introv (x&M). applys* triple_hforall. Qed.
+
+(** corrolary *)
+Lemma Triple_hforall_for : forall B (x:B) t (J:B->hprop) `{EA:Enc A} (Q:A->hprop),
+  Triple t (J x) Q ->
+  Triple t (hforall J) Q.
+Proof using. intros. applys* Triple_hforall. Qed.
+
+Lemma Triple_hprop : forall t (P:Prop) `{Enc A} H (Q:A->hprop),
+  (P -> Triple t H Q) ->
+  Triple t (\[P] \* H) Q.
+Proof using. intros. applys~ triple_hprop. Qed.
+
+Lemma Triple_hwand_hpure_l : forall t (P:Prop) H `{EA:Enc A} (Q:A->hprop),
+  P ->
+  Triple t H Q ->
+  Triple t (\[P] \-* H) Q.
+Proof using. unfold Triple. introv M N. applys* triple_hwand_hpure_l. Qed.
+
+Lemma Triple_frame : forall t `{Enc A} H (Q:A->hprop) H',
+  Triple t H Q ->
+  Triple t (H \* H') (Q \*+ H').
+Proof using.
+  introv M. unfold Triple. rewrite Post_star. applys* triple_frame.
+Qed.
+
+(*
+Lemma Triple_ramified_frame_htop : forall t `{Enc A} H H1 (Q1 Q:A->hprop),
+  Triple t H1 Q1 ->
+  H ==> H1 \* (Q1 \--* Q \*+ \Top) ->
+  Triple t H Q.
+Proof using. .. Qed.
+
+Lemma Triple_ramified_frame : forall t `{Enc A} H H1 (Q1 Q:A->hprop),
+  Triple t H1 Q1 ->
+  H ==> H1 \* (Q1 \--* Q) ->
+  Triple t H Q.
+Proof using. .. Qed.
+*)
+
+Lemma Triple_hor : forall t H1 H2 `{Enc A} (Q:A->hprop),
+  Triple t H1 Q ->
+  Triple t H2 Q ->
+  Triple t (hor H1 H2) Q.
+Proof using. introv M1 M2. applys* triple_hor. Qed.
+
+Lemma triple_hand_l : forall t H1 H2 `{Enc A} (Q:A->hprop),
+  Triple t H1 Q ->
+  Triple t (hand H1 H2) Q.
+Proof using. introv M1 M2. applys* triple_hand_l. Qed.
+
+Lemma Triple_hand_r : forall t H1 H2 `{Enc A} (Q:A->hprop),
+  Triple t H2 Q ->
+  Triple t (hand H1 H2) Q.
+Proof using. introv M1 M2. applys* triple_hand_r. Qed.
+
+Lemma Triple_htop_post : forall t `{Enc A} H (Q:A->hprop),
+  Triple t H (Q \*+ \Top) ->
+  Triple t H Q.
+Proof using.
+  introv M. unfolds Triple. rewrite Post_star in M. applys* triple_htop_post.
+Qed.
+
+Lemma Triple_htop_pre : forall t `{Enc A} H (Q:A->hprop),
+  Triple t H Q ->
+  Triple t (H \* \Top) Q.
+Proof using. introv M. applys* triple_htop_pre. Qed.
+
+Lemma Triple_combined : forall t H1 H2 `{Enc A} (Q1 Q:A->hprop) H,
+  Triple t H1 Q1 ->
+  H ==> H1 \* H2 ->
+  Q1 \*+ H2 ===> Q \*+ \Top ->
+  Triple t H Q.
+Proof using.
+  introv M WH WQ. applys* triple_combined. 
+  do 2 rewrite <- Post_star. apply* Post_himpl.
+Qed.
+
+End Structural.
