theories/LambdaSepLifted.v
@@ -629,6 +629,9 @@ Qed.
 (* ---------------------------------------------------------------------- *)
 (* ** Lifting of structural rules *)
 
+Section Structural.
+Hint Resolve is_local_Triple.
+
 Lemma Triple_conseq : forall t H' `{Enc A} (Q':A->hprop) H (Q:A->hprop),
   H ==> H' ->
   Triple t H' Q' ->
@@ -639,39 +642,52 @@ Proof using. introv MH M MQ. applys* triple_conseq MH. Qed.
 Lemma Triple_hexists : forall t `{Enc A} B (J:B->hprop) (Q:A->hprop),
   (forall x, Triple t (J x) Q) ->
   Triple t (hexists J) Q.
-Proof using. intros. applys~ triple_hexists. Qed.
+Proof using. intros. applys~ local_hexists. Qed.
 
-Lemma Triple_hforall : forall t B (J:B->hprop) `{EA:Enc A} (Q:A->hprop),
+Lemma Triple_hforall_exists : forall t B (J:B->hprop) `{EA:Enc A} (Q:A->hprop),
   (exists x, Triple t (J x) Q) ->
   Triple t (hforall J) Q.
-Proof using. unfold Triple. introv (x&M). applys* triple_hforall. Qed.
+Proof using. intros. applys~ local_hforall_exists. Qed.
 
-Lemma Triple_hforall_for : forall B (x:B) t (J:B->hprop) `{EA:Enc A} (Q:A->hprop),
+Lemma Triple_hforall : forall B (x:B) t (J:B->hprop) `{EA:Enc A} (Q:A->hprop),
   Triple t (J x) Q ->
   Triple t (hforall J) Q.
-Proof using. intros. applys* Triple_hforall. Qed.
-
-Lemma triple_hforall_for : forall A (x:A) t (J:A->hprop) Q,
-  triple t (J x) Q ->
-  triple t (hforall J) Q.
-Proof using. intros. applys* triple_hforall. Qed.
+Proof using. intros. applys~ local_hforall. Qed.
 
 Lemma Triple_hprop : forall t (P:Prop) `{Enc A} H (Q:A->hprop),
   (P -> Triple t H Q) ->
   Triple t (\[P] \* H) Q.
-Proof using. intros. applys~ triple_hprop. Qed.
+Proof using. intros. applys~ local_hprop. Qed.
+(* Proof using. intros. applys~ triple_hprop. Qed. *)
 
 Lemma Triple_hwand_hpure_l : forall t (P:Prop) H `{EA:Enc A} (Q:A->hprop),
   P ->
   Triple t H Q ->
   Triple t (\[P] \-* H) Q.
-Proof using. unfold Triple. introv M N. applys* triple_hwand_hpure_l. Qed.
+Proof using. intros. applys~ triple_hwand_hpure_l. Qed.
+(* Proof using. unfold Triple. introv M N. applys* triple_hwand_hpure_l. Qed. *)
 
 Lemma Triple_frame : forall t `{Enc A} H (Q:A->hprop) H',
   Triple t H Q ->
   Triple t (H \* H') (Q \*+ H').
 Proof using.
   introv M. unfold Triple. rewrite Post_star. applys* triple_frame.
+Qed.
+
+Lemma Triple_ramified_frame_htop : forall t `{Enc A} H H1 (Q1 Q:A->hprop),
+  Triple t H1 Q1 ->
+  H ==> H1 \* (Q1 \--* Q \*+ \Top) ->
+  Triple t H Q.
+Proof using.
+  introv M N. applys~ local_ramified_frame_htop M N.
+Qed.
+
+Lemma Triple_ramified_frame : forall t `{Enc A} H H1 (Q1 Q:A->hprop),
+  Triple t H1 Q1 ->
+  H ==> H1 \* (Q1 \--* Q) ->
+  Triple t H Q.
+Proof using.
+  introv M N. applys~ local_ramified_frame M N.
 Qed.
 
 Lemma Triple_hor : forall t H1 H2 `{Enc A} (Q:A->hprop),
@@ -693,14 +709,18 @@ Proof using. introv M1 M2. applys* triple_hand_r. Qed.
 Lemma Triple_htop_post : forall t `{Enc A} H (Q:A->hprop),
   Triple t H (Q \*+ \Top) ->
   Triple t H Q.
+Proof using. intros. applys* local_htop_post. Qed.
+(*
 Proof using.
   introv M. unfolds Triple. rewrite Post_star in M. applys* triple_htop_post.
 Qed.
+*)
 
 Lemma Triple_htop_pre : forall t `{Enc A} H (Q:A->hprop),
   Triple t H Q ->
   Triple t (H \* \Top) Q.
-Proof using. introv M. applys* triple_htop_pre. Qed.
+Proof using. intros. applys* local_htop_pre. Qed.
+(* Proof using. introv M. applys* triple_htop_pre. Qed. *)
 
 Lemma Triple_combined : forall t H1 H2 `{Enc A} (Q1 Q:A->hprop) H,
   Triple t H1 Q1 ->
@@ -711,6 +731,8 @@ Proof using.
   introv M WH WQ. applys* triple_combined. 
   do 2 rewrite <- Post_star. apply* Post_himpl.
 Qed.
+
+End Structural.
 
 
 (* ---------------------------------------------------------------------- *)
